hachi/lean/Generated.lean
@@ -708,7 +708,7 @@ structure ringswitch.RlinStatement where
   bound : Std.U64
 
 /-- [hachi::sumcheck::NestedZeroCheckStmt]
-    Source: 'src/sumcheck.rs', lines 1111:0-1117:1
+    Source: 'src/sumcheck.rs', lines 1119:0-1125:1
     Visibility: public -/
 structure sumcheck.NestedZeroCheckStmt where
   rlin : ringswitch.RlinStatement
@@ -718,7 +718,7 @@ structure sumcheck.NestedZeroCheckStmt where
   tau1 : alloc.vec.Vec cpoly.field.Ext4
 
 /-- [hachi::sumcheck::RoundStatement]
-    Source: 'src/sumcheck.rs', lines 1204:0-1209:1
+    Source: 'src/sumcheck.rs', lines 1212:0-1217:1
     Visibility: public -/
 structure sumcheck.RoundStatement where
   zc : sumcheck.NestedZeroCheckStmt
@@ -727,28 +727,28 @@ structure sumcheck.RoundStatement where
   target_alpha : cpoly.field.Ext4
 
 /-- [hachi::sumcheck::RoundMsg]
-    Source: 'src/sumcheck.rs', lines 1173:0-1176:1
+    Source: 'src/sumcheck.rs', lines 1181:0-1184:1
     Visibility: public -/
 structure sumcheck.RoundMsg where
   g_zero : cpoly.univariate.UnivariatePoly
   g_alpha : cpoly.univariate.UnivariatePoly
 
 /-- [hachi::sumcheck::{hachi::sumcheck::RoundMsg}::g_alpha]:
-    Source: 'src/sumcheck.rs', lines 1190:4-1192:5
+    Source: 'src/sumcheck.rs', lines 1198:4-1200:5
     Visibility: public -/
 def sumcheck.RoundMsg.impl.g_alpha
   (self : sumcheck.RoundMsg) : Result cpoly.univariate.UnivariatePoly := do
   ok self.g_alpha
 
 /-- [hachi::sumcheck::{hachi::sumcheck::RoundMsg}::g_zero]:
-    Source: 'src/sumcheck.rs', lines 1185:4-1187:5
+    Source: 'src/sumcheck.rs', lines 1193:4-1195:5
     Visibility: public -/
 def sumcheck.RoundMsg.impl.g_zero
   (self : sumcheck.RoundMsg) : Result cpoly.univariate.UnivariatePoly := do
   ok self.g_zero
 
 /-- [hachi::sumcheck::round_out]:
-    Source: 'src/sumcheck.rs', lines 1364:0-1375:1
+    Source: 'src/sumcheck.rs', lines 1372:0-1383:1
     Visibility: public -/
 def sumcheck.round_out
   (stmt : sumcheck.RoundStatement) (g : sumcheck.RoundMsg)
@@ -763,21 +763,21 @@ def sumcheck.round_out
   ok { stmt with challenges, target_zero, target_alpha }
 
 /-- [hachi::sumcheck::{hachi::sumcheck::RoundStatement}::target_alpha]:
-    Source: 'src/sumcheck.rs', lines 1243:4-1245:5
+    Source: 'src/sumcheck.rs', lines 1251:4-1253:5
     Visibility: public -/
 def sumcheck.RoundStatement.impl.target_alpha
   (self : sumcheck.RoundStatement) : Result cpoly.field.Ext4 := do
   ok self.target_alpha
 
 /-- [hachi::sumcheck::{hachi::sumcheck::RoundStatement}::target_zero]:
-    Source: 'src/sumcheck.rs', lines 1238:4-1240:5
+    Source: 'src/sumcheck.rs', lines 1246:4-1248:5
     Visibility: public -/
 def sumcheck.RoundStatement.impl.target_zero
   (self : sumcheck.RoundStatement) : Result cpoly.field.Ext4 := do
   ok self.target_zero
 
 /-- [hachi::sumcheck::round_check]:
-    Source: 'src/sumcheck.rs', lines 1348:0-1352:1
+    Source: 'src/sumcheck.rs', lines 1356:0-1360:1
     Visibility: public -/
 def sumcheck.round_check
   (stmt : sumcheck.RoundStatement) (g : sumcheck.RoundMsg) : Result Bool := do
@@ -798,14 +798,14 @@ def sumcheck.round_check
   else ok false
 
 /-- [hachi::sumcheck::{hachi::sumcheck::RoundStatement}::zc]:
-    Source: 'src/sumcheck.rs', lines 1228:4-1230:5
+    Source: 'src/sumcheck.rs', lines 1236:4-1238:5
     Visibility: public -/
 def sumcheck.RoundStatement.impl.zc
   (self : sumcheck.RoundStatement) : Result sumcheck.NestedZeroCheckStmt := do
   ok self.zc
 
 /-- [hachi::sumcheck::{hachi::sumcheck::NestedZeroCheckStmt}::tau0]:
-    Source: 'src/sumcheck.rs', lines 1154:4-1156:5
+    Source: 'src/sumcheck.rs', lines 1162:4-1164:5
     Visibility: public -/
 def sumcheck.NestedZeroCheckStmt.impl.tau0
   (self : sumcheck.NestedZeroCheckStmt) :
@@ -814,7 +814,7 @@ def sumcheck.NestedZeroCheckStmt.impl.tau0
   ok self.tau0
 
 /-- [hachi::sumcheck::round_verify_loop]: loop body 0:
-    Source: 'src/sumcheck.rs', lines 1601:4-1611:1
+    Source: 'src/sumcheck.rs', lines 1609:4-1619:1
     Visibility: public -/
 @[rust_loop_body]
 def sumcheck.round_verify_loop_loop.body
@@ -842,7 +842,7 @@ def sumcheck.round_verify_loop_loop.body
   else ok (done (some current))
 
 /-- [hachi::sumcheck::round_verify_loop]: loop 0:
-    Source: 'src/sumcheck.rs', lines 1601:4-1611:1
+    Source: 'src/sumcheck.rs', lines 1609:4-1619:1
     Visibility: public -/
 @[rust_loop]
 def sumcheck.round_verify_loop_loop
@@ -857,7 +857,7 @@ def sumcheck.round_verify_loop_loop
     (current, i)
 
 /-- [hachi::sumcheck::round_verify_loop]:
-    Source: 'src/sumcheck.rs', lines 1593:0-1611:1
+    Source: 'src/sumcheck.rs', lines 1601:0-1619:1
     Visibility: public -/
 def sumcheck.round_verify_loop
   (stmt : sumcheck.RoundStatement) (msgs : alloc.vec.Vec sumcheck.RoundMsg)
@@ -1093,7 +1093,7 @@ def zerocheck.zc_target_alpha
     0#usize
 
 /-- [hachi::sumcheck::{hachi::sumcheck::RoundStatement}::new]:
-    Source: 'src/sumcheck.rs', lines 1213:4-1225:5
+    Source: 'src/sumcheck.rs', lines 1221:4-1233:5
     Visibility: public -/
 def sumcheck.RoundStatement.new
   (zc : sumcheck.NestedZeroCheckStmt)
@@ -1104,7 +1104,7 @@ def sumcheck.RoundStatement.new
   ok { zc, challenges, target_zero, target_alpha }
 
 /-- [hachi::sumcheck::{hachi::sumcheck::NestedZeroCheckStmt}::tau1]:
-    Source: 'src/sumcheck.rs', lines 1159:4-1161:5
+    Source: 'src/sumcheck.rs', lines 1167:4-1169:5
     Visibility: public -/
 def sumcheck.NestedZeroCheckStmt.impl.tau1
   (self : sumcheck.NestedZeroCheckStmt) :
@@ -1113,21 +1113,21 @@ def sumcheck.NestedZeroCheckStmt.impl.tau1
   ok self.tau1
 
 /-- [hachi::sumcheck::{hachi::sumcheck::NestedZeroCheckStmt}::alpha]:
-    Source: 'src/sumcheck.rs', lines 1149:4-1151:5
+    Source: 'src/sumcheck.rs', lines 1157:4-1159:5
     Visibility: public -/
 def sumcheck.NestedZeroCheckStmt.impl.alpha
   (self : sumcheck.NestedZeroCheckStmt) : Result cpoly.field.Ext4 := do
   ok self.alpha
 
 /-- [hachi::sumcheck::{hachi::sumcheck::NestedZeroCheckStmt}::rlin]:
-    Source: 'src/sumcheck.rs', lines 1139:4-1141:5
+    Source: 'src/sumcheck.rs', lines 1147:4-1149:5
     Visibility: public -/
 def sumcheck.NestedZeroCheckStmt.impl.rlin
   (self : sumcheck.NestedZeroCheckStmt) : Result ringswitch.RlinStatement := do
   ok self.rlin
 
 /-- [hachi::sumcheck::nested_to_round_statement]:
-    Source: 'src/sumcheck.rs', lines 1492:0-1495:1
+    Source: 'src/sumcheck.rs', lines 1500:0-1503:1
     Visibility: public -/
 def sumcheck.nested_to_round_statement
   (zc : sumcheck.NestedZeroCheckStmt) : Result sumcheck.RoundStatement := do
@@ -1227,7 +1227,7 @@ def zerocheck.range_product
   cpoly.field.Ext4.Insts.CoreOpsArithMulExt4Ext4.mul v acc1
 
 /-- [hachi::sumcheck::{hachi::sumcheck::RoundStatement}::challenges]:
-    Source: 'src/sumcheck.rs', lines 1233:4-1235:5
+    Source: 'src/sumcheck.rs', lines 1241:4-1243:5
     Visibility: public -/
 def sumcheck.RoundStatement.impl.challenges
   (self : sumcheck.RoundStatement) :
@@ -1563,7 +1563,7 @@ def zerocheck.eq_weight_table
   zerocheck.eq_weight_table_loop tau1 n vars out 0#usize
 
 /-- [hachi::sumcheck::cube_size]: loop body 0:
-    Source: 'src/sumcheck.rs', lines 375:4-378:5 -/
+    Source: 'src/sumcheck.rs', lines 383:4-386:5 -/
 @[rust_loop_body]
 def sumcheck.cube_size_loop.body
   (vars : Std.Usize) (sz : Std.Usize) (k : Std.Usize) :
@@ -1576,7 +1576,7 @@ def sumcheck.cube_size_loop.body
   else ok (done sz)
 
 /-- [hachi::sumcheck::cube_size]: loop 0:
-    Source: 'src/sumcheck.rs', lines 375:4-378:5 -/
+    Source: 'src/sumcheck.rs', lines 383:4-386:5 -/
 @[rust_loop]
 def sumcheck.cube_size_loop
   (vars : Std.Usize) (sz : Std.Usize) (k : Std.Usize) : Result Std.Usize := do
@@ -1585,13 +1585,13 @@ def sumcheck.cube_size_loop
     (sz, k)
 
 /-- [hachi::sumcheck::cube_size]:
-    Source: 'src/sumcheck.rs', lines 372:0-380:1 -/
+    Source: 'src/sumcheck.rs', lines 380:0-388:1 -/
 @[reducible]
 def sumcheck.cube_size (vars : Std.Usize) : Result Std.Usize := do
   sumcheck.cube_size_loop vars 1#usize 0#usize
 
 /-- [hachi::sumcheck::alpha_public_mle_eval]: loop body 0:
-    Source: 'src/sumcheck.rs', lines 841:4-844:5
+    Source: 'src/sumcheck.rs', lines 849:4-852:5
     Visibility: public -/
 @[rust_loop_body]
 def sumcheck.alpha_public_mle_eval_loop0.body
@@ -1608,7 +1608,7 @@ def sumcheck.alpha_public_mle_eval_loop0.body
   else ok (done (k, sz))
 
 /-- [hachi::sumcheck::alpha_public_mle_eval]: loop 0:
-    Source: 'src/sumcheck.rs', lines 841:4-844:5
+    Source: 'src/sumcheck.rs', lines 849:4-852:5
     Visibility: public -/
 @[rust_loop]
 def sumcheck.alpha_public_mle_eval_loop0
@@ -1621,7 +1621,7 @@ def sumcheck.alpha_public_mle_eval_loop0
     (k, sz)
 
 /-- [hachi::sumcheck::alpha_public_mle_eval]: loop body 1:
-    Source: 'src/sumcheck.rs', lines 847:4-850:5
+    Source: 'src/sumcheck.rs', lines 855:4-858:5
     Visibility: public -/
 @[rust_loop_body]
 def sumcheck.alpha_public_mle_eval_loop1.body
@@ -1642,7 +1642,7 @@ def sumcheck.alpha_public_mle_eval_loop1.body
   else ok (done low)
 
 /-- [hachi::sumcheck::alpha_public_mle_eval]: loop 1:
-    Source: 'src/sumcheck.rs', lines 847:4-850:5
+    Source: 'src/sumcheck.rs', lines 855:4-858:5
     Visibility: public -/
 @[rust_loop]
 def sumcheck.alpha_public_mle_eval_loop1
@@ -1655,7 +1655,7 @@ def sumcheck.alpha_public_mle_eval_loop1
     (low, j)
 
 /-- [hachi::sumcheck::alpha_public_mle_eval]: loop body 3:
-    Source: 'src/sumcheck.rs', lines 859:8-864:9
+    Source: 'src/sumcheck.rs', lines 867:8-872:9
     Visibility: public -/
 @[rust_loop_body]
 def sumcheck.alpha_public_mle_eval_loop2_loop0.body
@@ -1687,7 +1687,7 @@ def sumcheck.alpha_public_mle_eval_loop2_loop0.body
   else ok (done sum)
 
 /-- [hachi::sumcheck::alpha_public_mle_eval]: loop 3:
-    Source: 'src/sumcheck.rs', lines 859:8-864:9
+    Source: 'src/sumcheck.rs', lines 867:8-872:9
     Visibility: public -/
 @[rust_loop]
 def sumcheck.alpha_public_mle_eval_loop2_loop0
@@ -1702,7 +1702,7 @@ def sumcheck.alpha_public_mle_eval_loop2_loop0
     (sum, i)
 
 /-- [hachi::sumcheck::alpha_public_mle_eval]: loop body 2:
-    Source: 'src/sumcheck.rs', lines 856:4-867:5
+    Source: 'src/sumcheck.rs', lines 864:4-875:5
     Visibility: public -/
 @[rust_loop_body]
 def sumcheck.alpha_public_mle_eval_loop2.body
@@ -1724,7 +1724,7 @@ def sumcheck.alpha_public_mle_eval_loop2.body
   else ok (done high)
 
 /-- [hachi::sumcheck::alpha_public_mle_eval]: loop 2:
-    Source: 'src/sumcheck.rs', lines 856:4-867:5
+    Source: 'src/sumcheck.rs', lines 864:4-875:5
     Visibility: public -/
 @[rust_loop]
 def sumcheck.alpha_public_mle_eval_loop2
@@ -1740,7 +1740,7 @@ def sumcheck.alpha_public_mle_eval_loop2
     (high, u)
 
 /-- [hachi::sumcheck::alpha_public_mle_eval]: loop body 4:
-    Source: 'src/sumcheck.rs', lines 869:4-872:5
+    Source: 'src/sumcheck.rs', lines 877:4-880:5
     Visibility: public -/
 @[rust_loop_body]
 def sumcheck.alpha_public_mle_eval_loop3.body
@@ -1761,7 +1761,7 @@ def sumcheck.alpha_public_mle_eval_loop3.body
   else ok (done high)
 
 /-- [hachi::sumcheck::alpha_public_mle_eval]: loop 4:
-    Source: 'src/sumcheck.rs', lines 869:4-872:5
+    Source: 'src/sumcheck.rs', lines 877:4-880:5
     Visibility: public -/
 @[rust_loop]
 def sumcheck.alpha_public_mle_eval_loop3
@@ -1775,7 +1775,7 @@ def sumcheck.alpha_public_mle_eval_loop3
     (high, j2)
 
 /-- [hachi::sumcheck::alpha_public_mle_eval]:
-    Source: 'src/sumcheck.rs', lines 829:0-874:1
+    Source: 'src/sumcheck.rs', lines 837:0-882:1
     Visibility: public -/
 def sumcheck.alpha_public_mle_eval
   (s : ringswitch.RlinStatement) (alpha : cpoly.field.Ext4)
@@ -1810,7 +1810,7 @@ def sumcheck.alpha_public_mle_eval
   cpoly.field.Ext4.Insts.CoreOpsArithMulExt4Ext4.mul e e1
 
 /-- [hachi::sumcheck::eq_prefix]: loop body 0:
-    Source: 'src/sumcheck.rs', lines 401:4-406:5
+    Source: 'src/sumcheck.rs', lines 409:4-414:5
     Visibility: public -/
 @[rust_loop_body]
 def sumcheck.eq_prefix_loop.body
@@ -1840,7 +1840,7 @@ def sumcheck.eq_prefix_loop.body
   else ok (done acc)
 
 /-- [hachi::sumcheck::eq_prefix]: loop 0:
-    Source: 'src/sumcheck.rs', lines 401:4-406:5
+    Source: 'src/sumcheck.rs', lines 409:4-414:5
     Visibility: public -/
 @[rust_loop]
 def sumcheck.eq_prefix_loop
@@ -1854,7 +1854,7 @@ def sumcheck.eq_prefix_loop
     (acc, k)
 
 /-- [hachi::sumcheck::eq_prefix]:
-    Source: 'src/sumcheck.rs', lines 397:0-408:1
+    Source: 'src/sumcheck.rs', lines 405:0-416:1
     Visibility: public -/
 def sumcheck.eq_prefix
   (tau0 : alloc.vec.Vec cpoly.field.Ext4)
@@ -1872,7 +1872,7 @@ def ringswitch.RlinStatement.impl.bound
   ok self.bound
 
 /-- [hachi::sumcheck::final_check]:
-    Source: 'src/sumcheck.rs', lines 1418:0-1425:1
+    Source: 'src/sumcheck.rs', lines 1426:0-1433:1
     Visibility: public -/
 def sumcheck.final_check
   (stmt : sumcheck.RoundStatement) (y_prime : cpoly.field.Ext4)
@@ -1903,7 +1903,7 @@ def sumcheck.final_check
   else ok false
 
 /-- [hachi::sumcheck::{hachi::sumcheck::NestedZeroCheckStmt}::new]:
-    Source: 'src/sumcheck.rs', lines 1122:4-1136:5
+    Source: 'src/sumcheck.rs', lines 1130:4-1144:5
     Visibility: public -/
 def sumcheck.NestedZeroCheckStmt.new
   (rlin : ringswitch.RlinStatement) (t : linalg.PolyVec)
@@ -5399,7 +5399,7 @@ def zerocheck.c_w_table_fp
   zerocheck.c_w_table_fp_loop0 w size params.RING_DEGREE values 0#usize 0#usize
 
 /-- [hachi::sumcheck::poly_mul]: loop body 1:
-    Source: 'src/sumcheck.rs', lines 1090:8-1095:9
+    Source: 'src/sumcheck.rs', lines 1098:8-1103:9
     Visibility: public -/
 @[rust_loop_body]
 def sumcheck.poly_mul_loop0_loop0.body
@@ -5432,7 +5432,7 @@ def sumcheck.poly_mul_loop0_loop0.body
   else ok (done out)
 
 /-- [hachi::sumcheck::poly_mul]: loop 1:
-    Source: 'src/sumcheck.rs', lines 1090:8-1095:9
+    Source: 'src/sumcheck.rs', lines 1098:8-1103:9
     Visibility: public -/
 @[rust_loop]
 def sumcheck.poly_mul_loop0_loop0
@@ -5446,7 +5446,7 @@ def sumcheck.poly_mul_loop0_loop0
     (out, j)
 
 /-- [hachi::sumcheck::poly_mul]: loop body 0:
-    Source: 'src/sumcheck.rs', lines 1088:4-1097:5
+    Source: 'src/sumcheck.rs', lines 1096:4-1105:5
     Visibility: public -/
 @[rust_loop_body]
 def sumcheck.poly_mul_loop0.body
@@ -5464,7 +5464,7 @@ def sumcheck.poly_mul_loop0.body
   else ok (done out)
 
 /-- [hachi::sumcheck::poly_mul]: loop 0:
-    Source: 'src/sumcheck.rs', lines 1088:4-1097:5
+    Source: 'src/sumcheck.rs', lines 1096:4-1105:5
     Visibility: public -/
 @[rust_loop]
 def sumcheck.poly_mul_loop0
@@ -5478,7 +5478,7 @@ def sumcheck.poly_mul_loop0
     (out, i)
 
 /-- [hachi::sumcheck::poly_mul]:
-    Source: 'src/sumcheck.rs', lines 1080:0-1099:1
+    Source: 'src/sumcheck.rs', lines 1088:0-1107:1
     Visibility: public -/
 def sumcheck.poly_mul
   (a : cpoly.univariate.UnivariatePoly) (b : cpoly.univariate.UnivariatePoly) :
@@ -5502,7 +5502,7 @@ def sumcheck.poly_mul
       cpoly.univariate.UnivariatePoly.trim up
 
 /-- [hachi::sumcheck::round_value_alpha_base_split]: loop body 0:
-    Source: 'src/sumcheck.rs', lines 1018:4-1025:5
+    Source: 'src/sumcheck.rs', lines 1026:4-1033:5
     Visibility: public -/
 @[rust_loop_body]
 def sumcheck.round_value_alpha_base_split_loop.body
@@ -5558,7 +5558,7 @@ def sumcheck.round_value_alpha_base_split_loop.body
   else ok (done acc)
 
 /-- [hachi::sumcheck::round_value_alpha_base_split]: loop 0:
-    Source: 'src/sumcheck.rs', lines 1018:4-1025:5
+    Source: 'src/sumcheck.rs', lines 1026:4-1033:5
     Visibility: public -/
 @[rust_loop]
 def sumcheck.round_value_alpha_base_split_loop
@@ -5575,7 +5575,7 @@ def sumcheck.round_value_alpha_base_split_loop
     (acc, y)
 
 /-- [hachi::sumcheck::round_value_alpha_base_split]:
-    Source: 'src/sumcheck.rs', lines 1005:0-1027:1
+    Source: 'src/sumcheck.rs', lines 1013:0-1035:1
     Visibility: public -/
 def sumcheck.round_value_alpha_base_split
   (w : alloc.vec.Vec cpoly.field.Fp) (low : alloc.vec.Vec cpoly.field.Ext4)
@@ -5601,7 +5601,7 @@ def sumcheck.round_value_alpha_base_split
 def params.ROUND_NODES_ALPHA : Std.Usize := 3#usize
 
 /-- [hachi::sumcheck::round_values_alpha_base_split]: loop body 0:
-    Source: 'src/sumcheck.rs', lines 1034:4-1037:5
+    Source: 'src/sumcheck.rs', lines 1042:4-1045:5
     Visibility: public -/
 @[rust_loop_body]
 def sumcheck.round_values_alpha_base_split_loop.body
@@ -5622,7 +5622,7 @@ def sumcheck.round_values_alpha_base_split_loop.body
   else ok (done out)
 
 /-- [hachi::sumcheck::round_values_alpha_base_split]: loop 0:
-    Source: 'src/sumcheck.rs', lines 1034:4-1037:5
+    Source: 'src/sumcheck.rs', lines 1042:4-1045:5
     Visibility: public -/
 @[rust_loop]
 def sumcheck.round_values_alpha_base_split_loop
@@ -5637,7 +5637,7 @@ def sumcheck.round_values_alpha_base_split_loop
     (out, t)
 
 /-- [hachi::sumcheck::round_values_alpha_base_split]:
-    Source: 'src/sumcheck.rs', lines 1030:0-1039:1
+    Source: 'src/sumcheck.rs', lines 1038:0-1047:1
     Visibility: public -/
 @[reducible]
 def sumcheck.round_values_alpha_base_split
@@ -5656,7 +5656,7 @@ def params.ROUND_NODE_INV_ALPHA : Array Std.U64 3#usize :=
   Array.make 3#usize [ 2147483599#u64, 4294967196#u64, 2147483599#u64 ]
 
 /-- [hachi::sumcheck::round_node_weights_alpha]: loop body 0:
-    Source: 'src/sumcheck.rs', lines 520:4-523:5
+    Source: 'src/sumcheck.rs', lines 528:4-531:5
     Visibility: public -/
 @[rust_loop_body]
 def sumcheck.round_node_weights_alpha_loop.body
@@ -5674,7 +5674,7 @@ def sumcheck.round_node_weights_alpha_loop.body
   else ok (done out)
 
 /-- [hachi::sumcheck::round_node_weights_alpha]: loop 0:
-    Source: 'src/sumcheck.rs', lines 520:4-523:5
+    Source: 'src/sumcheck.rs', lines 528:4-531:5
     Visibility: public -/
 @[rust_loop]
 def sumcheck.round_node_weights_alpha_loop
@@ -5686,7 +5686,7 @@ def sumcheck.round_node_weights_alpha_loop
     (out, i)
 
 /-- [hachi::sumcheck::round_node_weights_alpha]:
-    Source: 'src/sumcheck.rs', lines 516:0-525:1
+    Source: 'src/sumcheck.rs', lines 524:0-533:1
     Visibility: public -/
 @[reducible]
 def sumcheck.round_node_weights_alpha
@@ -5923,7 +5923,7 @@ def sumcheck.interpolate
   cpoly.univariate.UnivariatePoly.from_coeffs acc1
 
 /-- [hachi::sumcheck::round_poly_alpha_base_split]:
-    Source: 'src/sumcheck.rs', lines 1042:0-1046:1
+    Source: 'src/sumcheck.rs', lines 1050:0-1054:1
     Visibility: public -/
 def sumcheck.round_poly_alpha_base_split
   (w : alloc.vec.Vec cpoly.field.Fp) (low : alloc.vec.Vec cpoly.field.Ext4)
@@ -6039,7 +6039,7 @@ def params.SHIFT_T : Array Std.U64 512#usize :=
 @[global_simps, irreducible] def params.SHIFT_DEG : Std.Usize := 32#usize
 
 /-- [hachi::sumcheck::shift_inner_base]: loop body 0:
-    Source: 'src/sumcheck.rs', lines 654:4-658:5
+    Source: 'src/sumcheck.rs', lines 662:4-666:5
     Visibility: public -/
 @[rust_loop_body]
 def sumcheck.shift_inner_base_loop.body
@@ -6066,7 +6066,7 @@ def sumcheck.shift_inner_base_loop.body
   else ok (done s)
 
 /-- [hachi::sumcheck::shift_inner_base]: loop 0:
-    Source: 'src/sumcheck.rs', lines 654:4-658:5
+    Source: 'src/sumcheck.rs', lines 662:4-666:5
     Visibility: public -/
 @[rust_loop]
 def sumcheck.shift_inner_base_loop
@@ -6079,7 +6079,7 @@ def sumcheck.shift_inner_base_loop
     (s, j)
 
 /-- [hachi::sumcheck::shift_inner_base]:
-    Source: 'src/sumcheck.rs', lines 649:0-660:1
+    Source: 'src/sumcheck.rs', lines 657:0-668:1
     Visibility: public -/
 def sumcheck.shift_inner_base
   (lop : alloc.vec.Vec cpoly.field.Fp) (m : Std.Usize) :
@@ -6090,7 +6090,7 @@ def sumcheck.shift_inner_base
     cpoly.field.Fp.ZERO j
 
 /-- [hachi::sumcheck::shift_accum_base]: loop body 0:
-    Source: 'src/sumcheck.rs', lines 668:4-675:5
+    Source: 'src/sumcheck.rs', lines 676:4-683:5
     Visibility: public -/
 @[rust_loop_body]
 def sumcheck.shift_accum_base_loop.body
@@ -6119,7 +6119,7 @@ def sumcheck.shift_accum_base_loop.body
   else ok (done acc)
 
 /-- [hachi::sumcheck::shift_accum_base]: loop 0:
-    Source: 'src/sumcheck.rs', lines 668:4-675:5
+    Source: 'src/sumcheck.rs', lines 676:4-683:5
     Visibility: public -/
 @[rust_loop]
 def sumcheck.shift_accum_base_loop
@@ -6134,7 +6134,7 @@ def sumcheck.shift_accum_base_loop
     (acc, dpow, m)
 
 /-- [hachi::sumcheck::shift_accum_base]:
-    Source: 'src/sumcheck.rs', lines 664:0-677:1
+    Source: 'src/sumcheck.rs', lines 672:0-685:1
     Visibility: public -/
 @[reducible]
 def sumcheck.shift_accum_base
@@ -6146,7 +6146,7 @@ def sumcheck.shift_accum_base
     cpoly.field.Fp.ONE 0#usize
 
 /-- [hachi::sumcheck::shift_powers_base]: loop body 0:
-    Source: 'src/sumcheck.rs', lines 640:4-644:5
+    Source: 'src/sumcheck.rs', lines 648:4-652:5
     Visibility: public -/
 @[rust_loop_body]
 def sumcheck.shift_powers_base_loop.body
@@ -6164,7 +6164,7 @@ def sumcheck.shift_powers_base_loop.body
   else ok (done out)
 
 /-- [hachi::sumcheck::shift_powers_base]: loop 0:
-    Source: 'src/sumcheck.rs', lines 640:4-644:5
+    Source: 'src/sumcheck.rs', lines 648:4-652:5
     Visibility: public -/
 @[rust_loop]
 def sumcheck.shift_powers_base_loop
@@ -6178,7 +6178,7 @@ def sumcheck.shift_powers_base_loop
     (out, cur, k)
 
 /-- [hachi::sumcheck::shift_powers_base]:
-    Source: 'src/sumcheck.rs', lines 635:0-646:1
+    Source: 'src/sumcheck.rs', lines 643:0-654:1
     Visibility: public -/
 def sumcheck.shift_powers_base
   (x : cpoly.field.Fp) : Result (alloc.vec.Vec cpoly.field.Fp) := do
@@ -6192,7 +6192,7 @@ def sumcheck.shift_powers_base
 @[global_simps, irreducible] def params.ROUND_NODES : Std.Usize := 33#usize
 
 /-- [hachi::sumcheck::round_poly_zero_base]: loop body 0:
-    Source: 'src/sumcheck.rs', lines 618:4-621:5
+    Source: 'src/sumcheck.rs', lines 626:4-629:5
     Visibility: public -/
 @[rust_loop_body]
 def sumcheck.round_poly_zero_base_loop0.body
@@ -6208,7 +6208,7 @@ def sumcheck.round_poly_zero_base_loop0.body
   else ok (done acc)
 
 /-- [hachi::sumcheck::round_poly_zero_base]: loop 0:
-    Source: 'src/sumcheck.rs', lines 618:4-621:5
+    Source: 'src/sumcheck.rs', lines 626:4-629:5
     Visibility: public -/
 @[rust_loop]
 def sumcheck.round_poly_zero_base_loop0
@@ -6220,7 +6220,7 @@ def sumcheck.round_poly_zero_base_loop0
     (acc, i)
 
 /-- [hachi::sumcheck::round_poly_zero_base]: loop body 1:
-    Source: 'src/sumcheck.rs', lines 623:4-629:5
+    Source: 'src/sumcheck.rs', lines 631:4-637:5
     Visibility: public -/
 @[rust_loop_body]
 def sumcheck.round_poly_zero_base_loop1.body
@@ -6250,7 +6250,7 @@ def sumcheck.round_poly_zero_base_loop1.body
   else ok (done acc)
 
 /-- [hachi::sumcheck::round_poly_zero_base]: loop 1:
-    Source: 'src/sumcheck.rs', lines 623:4-629:5
+    Source: 'src/sumcheck.rs', lines 631:4-637:5
     Visibility: public -/
 @[rust_loop]
 def sumcheck.round_poly_zero_base_loop1
@@ -6264,7 +6264,7 @@ def sumcheck.round_poly_zero_base_loop1
     (acc, y)
 
 /-- [hachi::sumcheck::round_poly_zero_base]:
-    Source: 'src/sumcheck.rs', lines 607:0-632:1
+    Source: 'src/sumcheck.rs', lines 615:0-640:1
     Visibility: public -/
 def sumcheck.round_poly_zero_base
   (w : alloc.vec.Vec cpoly.field.Fp) (eq : alloc.vec.Vec cpoly.field.Ext4) :
@@ -6278,7 +6278,7 @@ def sumcheck.round_poly_zero_base
   cpoly.univariate.UnivariatePoly.from_coeffs acc3
 
 /-- [hachi::sumcheck::eq_free_factor]:
-    Source: 'src/sumcheck.rs', lines 464:0-469:1
+    Source: 'src/sumcheck.rs', lines 472:0-477:1
     Visibility: public -/
 def sumcheck.eq_free_factor
   (t : cpoly.field.Ext4) : Result cpoly.univariate.UnivariatePoly := do
@@ -6292,7 +6292,7 @@ def sumcheck.eq_free_factor
   cpoly.univariate.UnivariatePoly.from_coeffs coeffs1
 
 /-- [hachi::sumcheck::eq_suffix_table]: loop body 1:
-    Source: 'src/sumcheck.rs', lines 437:8-440:9
+    Source: 'src/sumcheck.rs', lines 445:8-448:9
     Visibility: public -/
 @[rust_loop_body]
 def sumcheck.eq_suffix_table_loop0_loop0.body
@@ -6313,7 +6313,7 @@ def sumcheck.eq_suffix_table_loop0_loop0.body
   else ok (done next)
 
 /-- [hachi::sumcheck::eq_suffix_table]: loop 1:
-    Source: 'src/sumcheck.rs', lines 437:8-440:9
+    Source: 'src/sumcheck.rs', lines 445:8-448:9
     Visibility: public -/
 @[rust_loop]
 def sumcheck.eq_suffix_table_loop0_loop0
@@ -6327,7 +6327,7 @@ def sumcheck.eq_suffix_table_loop0_loop0
     (next, j)
 
 /-- [hachi::sumcheck::eq_suffix_table]: loop body 2:
-    Source: 'src/sumcheck.rs', lines 442:8-445:9
+    Source: 'src/sumcheck.rs', lines 450:8-453:9
     Visibility: public -/
 @[rust_loop_body]
 def sumcheck.eq_suffix_table_loop0_loop1.body
@@ -6348,7 +6348,7 @@ def sumcheck.eq_suffix_table_loop0_loop1.body
   else ok (done next)
 
 /-- [hachi::sumcheck::eq_suffix_table]: loop 2:
-    Source: 'src/sumcheck.rs', lines 442:8-445:9
+    Source: 'src/sumcheck.rs', lines 450:8-453:9
     Visibility: public -/
 @[rust_loop]
 def sumcheck.eq_suffix_table_loop0_loop1
@@ -6362,7 +6362,7 @@ def sumcheck.eq_suffix_table_loop0_loop1
     (next, j2)
 
 /-- [hachi::sumcheck::eq_suffix_table]: loop body 0:
-    Source: 'src/sumcheck.rs', lines 431:4-448:5
+    Source: 'src/sumcheck.rs', lines 439:4-456:5
     Visibility: public -/
 @[rust_loop_body]
 def sumcheck.eq_suffix_table_loop0.body
@@ -6388,7 +6388,7 @@ def sumcheck.eq_suffix_table_loop0.body
   else ok (done tab)
 
 /-- [hachi::sumcheck::eq_suffix_table]: loop 0:
-    Source: 'src/sumcheck.rs', lines 431:4-448:5
+    Source: 'src/sumcheck.rs', lines 439:4-456:5
     Visibility: public -/
 @[rust_loop]
 def sumcheck.eq_suffix_table_loop0
@@ -6401,7 +6401,7 @@ def sumcheck.eq_suffix_table_loop0
     (tab, k)
 
 /-- [hachi::sumcheck::eq_suffix_table]:
-    Source: 'src/sumcheck.rs', lines 426:0-450:1
+    Source: 'src/sumcheck.rs', lines 434:0-458:1
     Visibility: public -/
 def sumcheck.eq_suffix_table
   (tau0 : alloc.vec.Vec cpoly.field.Ext4) (i : Std.Usize) :
@@ -6415,7 +6415,7 @@ def sumcheck.eq_suffix_table
   sumcheck.eq_suffix_table_loop0 tau0 m0 tab k
 
 /-- [hachi::sumcheck::honest_compute_g_base_split]:
-    Source: 'src/sumcheck.rs', lines 1323:0-1338:1
+    Source: 'src/sumcheck.rs', lines 1331:0-1346:1
     Visibility: public -/
 def sumcheck.honest_compute_g_base_split
   (stmt : sumcheck.RoundStatement) (w_fp : alloc.vec.Vec cpoly.field.Fp)
@@ -6441,7 +6441,7 @@ def sumcheck.honest_compute_g_base_split
   ok { g_zero, g_alpha }
 
 /-- [hachi::sumcheck::round_value_alpha_split]: loop body 0:
-    Source: 'src/sumcheck.rs', lines 973:4-980:5
+    Source: 'src/sumcheck.rs', lines 981:4-988:5
     Visibility: public -/
 @[rust_loop_body]
 def sumcheck.round_value_alpha_split_loop.body
@@ -6496,7 +6496,7 @@ def sumcheck.round_value_alpha_split_loop.body
   else ok (done acc)
 
 /-- [hachi::sumcheck::round_value_alpha_split]: loop 0:
-    Source: 'src/sumcheck.rs', lines 973:4-980:5
+    Source: 'src/sumcheck.rs', lines 981:4-988:5
     Visibility: public -/
 @[rust_loop]
 def sumcheck.round_value_alpha_split_loop
@@ -6512,7 +6512,7 @@ def sumcheck.round_value_alpha_split_loop
     (acc, y)
 
 /-- [hachi::sumcheck::round_value_alpha_split]:
-    Source: 'src/sumcheck.rs', lines 962:0-982:1
+    Source: 'src/sumcheck.rs', lines 970:0-990:1
     Visibility: public -/
 def sumcheck.round_value_alpha_split
   (w : alloc.vec.Vec cpoly.field.Ext4) (low : alloc.vec.Vec cpoly.field.Ext4)
@@ -6529,7 +6529,7 @@ def sumcheck.round_value_alpha_split
     cpoly.field.Ext4.ZERO 0#usize
 
 /-- [hachi::sumcheck::round_values_alpha_split]: loop body 0:
-    Source: 'src/sumcheck.rs', lines 989:4-992:5
+    Source: 'src/sumcheck.rs', lines 997:4-1000:5
     Visibility: public -/
 @[rust_loop_body]
 def sumcheck.round_values_alpha_split_loop.body
@@ -6549,7 +6549,7 @@ def sumcheck.round_values_alpha_split_loop.body
   else ok (done out)
 
 /-- [hachi::sumcheck::round_values_alpha_split]: loop 0:
-    Source: 'src/sumcheck.rs', lines 989:4-992:5
+    Source: 'src/sumcheck.rs', lines 997:4-1000:5
     Visibility: public -/
 @[rust_loop]
 def sumcheck.round_values_alpha_split_loop
@@ -6564,7 +6564,7 @@ def sumcheck.round_values_alpha_split_loop
     (out, t)
 
 /-- [hachi::sumcheck::round_values_alpha_split]:
-    Source: 'src/sumcheck.rs', lines 985:0-994:1
+    Source: 'src/sumcheck.rs', lines 993:0-1002:1
     Visibility: public -/
 @[reducible]
 def sumcheck.round_values_alpha_split
@@ -6576,7 +6576,7 @@ def sumcheck.round_values_alpha_split
     (alloc.vec.Vec.new cpoly.field.Ext4) 0#usize
 
 /-- [hachi::sumcheck::round_poly_alpha_split]:
-    Source: 'src/sumcheck.rs', lines 997:0-1001:1
+    Source: 'src/sumcheck.rs', lines 1005:0-1009:1
     Visibility: public -/
 def sumcheck.round_poly_alpha_split
   (w : alloc.vec.Vec cpoly.field.Ext4) (low : alloc.vec.Vec cpoly.field.Ext4)
@@ -6639,51 +6639,50 @@ def sumcheck.shift_inner
     cpoly.field.Ext4.ZERO j
 
 /-- [hachi::sumcheck::shift_accum]: loop body 0:
-    Source: 'src/sumcheck.rs', lines 310:4-315:5
+    Source: 'src/sumcheck.rs', lines 317:4-323:5
     Visibility: public -/
 @[rust_loop_body]
 def sumcheck.shift_accum_loop.body
-  (lop : alloc.vec.Vec cpoly.field.Ext4) (d : cpoly.field.Ext4)
-  (e : cpoly.field.Ext4) (n : Std.Usize) (acc : alloc.vec.Vec cpoly.field.Ext4)
-  (dpow : cpoly.field.Ext4) (m : Std.Usize) :
+  (lop : alloc.vec.Vec cpoly.field.Ext4) (d : cpoly.field.Ext4) (n : Std.Usize)
+  (acc : alloc.vec.Vec cpoly.field.Ext4) (epow : cpoly.field.Ext4)
+  (m : Std.Usize) :
   Result (ControlFlow ((alloc.vec.Vec cpoly.field.Ext4) × cpoly.field.Ext4 ×
     Std.Usize) (alloc.vec.Vec cpoly.field.Ext4))
   := do
   if m < n
   then
     let s ← sumcheck.shift_inner lop m
-    let e1 ←
+    let cur ←
       alloc.vec.Vec.index (core.slice.index.SliceIndexUsizeSlice
         cpoly.field.Ext4) acc m
-    let e2 ← cpoly.field.Ext4.Insts.CoreOpsArithMulExt4Ext4.mul dpow s
-    let e3 ← cpoly.field.Ext4.Insts.CoreOpsArithMulExt4Ext4.mul e e2
-    let e4 ← cpoly.field.Ext4.Insts.CoreOpsArithAddExt4Ext4.add e1 e3
+    let e ← cpoly.field.Ext4.Insts.CoreOpsArithMulExt4Ext4.mul epow s
+    let e1 ← cpoly.field.Ext4.Insts.CoreOpsArithAddExt4Ext4.add cur e
     let (_, index_mut_back) ←
       alloc.vec.Vec.index_mut (core.slice.index.SliceIndexUsizeSlice
         cpoly.field.Ext4) acc m
-    let dpow1 ← cpoly.field.Ext4.Insts.CoreOpsArithMulExt4Ext4.mul dpow d
+    let epow1 ← cpoly.field.Ext4.Insts.CoreOpsArithMulExt4Ext4.mul epow d
     let m1 ← m + 1#usize
-    let acc1 := index_mut_back e4
-    ok (cont (acc1, dpow1, m1))
+    let acc1 := index_mut_back e1
+    ok (cont (acc1, epow1, m1))
   else ok (done acc)
 
 /-- [hachi::sumcheck::shift_accum]: loop 0:
-    Source: 'src/sumcheck.rs', lines 310:4-315:5
+    Source: 'src/sumcheck.rs', lines 317:4-323:5
     Visibility: public -/
 @[rust_loop]
 def sumcheck.shift_accum_loop
   (acc : alloc.vec.Vec cpoly.field.Ext4) (lop : alloc.vec.Vec cpoly.field.Ext4)
-  (d : cpoly.field.Ext4) (e : cpoly.field.Ext4) (n : Std.Usize)
-  (dpow : cpoly.field.Ext4) (m : Std.Usize) :
+  (d : cpoly.field.Ext4) (n : Std.Usize) (epow : cpoly.field.Ext4)
+  (m : Std.Usize) :
   Result (alloc.vec.Vec cpoly.field.Ext4)
   := do
   loop
-    (fun (acc1, dpow1, m1) => sumcheck.shift_accum_loop.body lop d e n acc1
-      dpow1 m1)
-    (acc, dpow, m)
+    (fun (acc1, epow1, m1) => sumcheck.shift_accum_loop.body lop d n acc1 epow1
+      m1)
+    (acc, epow, m)
 
 /-- [hachi::sumcheck::shift_accum]:
-    Source: 'src/sumcheck.rs', lines 306:0-317:1
+    Source: 'src/sumcheck.rs', lines 306:0-325:1
     Visibility: public -/
 @[reducible]
 def sumcheck.shift_accum
@@ -6691,8 +6690,7 @@ def sumcheck.shift_accum
   (d : cpoly.field.Ext4) (e : cpoly.field.Ext4) :
   Result (alloc.vec.Vec cpoly.field.Ext4)
   := do
-  sumcheck.shift_accum_loop acc lop d e params.SHIFT_DEG cpoly.field.Ext4.ONE
-    0#usize
+  sumcheck.shift_accum_loop acc lop d params.SHIFT_DEG e 0#usize
 
 /-- [hachi::sumcheck::shift_powers]: loop body 0:
     Source: 'src/sumcheck.rs', lines 263:4-267:5
@@ -6735,7 +6733,7 @@ def sumcheck.shift_powers
     0#usize
 
 /-- [hachi::sumcheck::round_poly_zero]: loop body 0:
-    Source: 'src/sumcheck.rs', lines 349:4-352:5
+    Source: 'src/sumcheck.rs', lines 357:4-360:5
     Visibility: public -/
 @[rust_loop_body]
 def sumcheck.round_poly_zero_loop0.body
@@ -6751,7 +6749,7 @@ def sumcheck.round_poly_zero_loop0.body
   else ok (done acc)
 
 /-- [hachi::sumcheck::round_poly_zero]: loop 0:
-    Source: 'src/sumcheck.rs', lines 349:4-352:5
+    Source: 'src/sumcheck.rs', lines 357:4-360:5
     Visibility: public -/
 @[rust_loop]
 def sumcheck.round_poly_zero_loop0
@@ -6763,7 +6761,7 @@ def sumcheck.round_poly_zero_loop0
     (acc, i)
 
 /-- [hachi::sumcheck::round_poly_zero]: loop body 1:
-    Source: 'src/sumcheck.rs', lines 354:4-360:5
+    Source: 'src/sumcheck.rs', lines 362:4-368:5
     Visibility: public -/
 @[rust_loop_body]
 def sumcheck.round_poly_zero_loop1.body
@@ -6793,7 +6791,7 @@ def sumcheck.round_poly_zero_loop1.body
   else ok (done acc)
 
 /-- [hachi::sumcheck::round_poly_zero]: loop 1:
-    Source: 'src/sumcheck.rs', lines 354:4-360:5
+    Source: 'src/sumcheck.rs', lines 362:4-368:5
     Visibility: public -/
 @[rust_loop]
 def sumcheck.round_poly_zero_loop1
@@ -6806,7 +6804,7 @@ def sumcheck.round_poly_zero_loop1
     (acc, y)
 
 /-- [hachi::sumcheck::round_poly_zero]:
-    Source: 'src/sumcheck.rs', lines 344:0-363:1
+    Source: 'src/sumcheck.rs', lines 352:0-371:1
     Visibility: public -/
 def sumcheck.round_poly_zero
   (w : alloc.vec.Vec cpoly.field.Ext4) (eq : alloc.vec.Vec cpoly.field.Ext4) :
@@ -6820,7 +6818,7 @@ def sumcheck.round_poly_zero
   cpoly.univariate.UnivariatePoly.from_coeffs acc3
 
 /-- [hachi::sumcheck::honest_compute_g_split]:
-    Source: 'src/sumcheck.rs', lines 1304:0-1320:1
+    Source: 'src/sumcheck.rs', lines 1312:0-1328:1
     Visibility: public -/
 def sumcheck.honest_compute_g_split
   (stmt : sumcheck.RoundStatement) (w_tab : alloc.vec.Vec cpoly.field.Ext4)
@@ -6846,7 +6844,7 @@ def sumcheck.honest_compute_g_split
   ok { g_zero, g_alpha }
 
 /-- [hachi::sumcheck::alpha_split_fold]:
-    Source: 'src/sumcheck.rs', lines 949:0-957:1
+    Source: 'src/sumcheck.rs', lines 957:0-965:1
     Visibility: public -/
 def sumcheck.alpha_split_fold
   (low : alloc.vec.Vec cpoly.field.Ext4)
@@ -6865,7 +6863,7 @@ def sumcheck.alpha_split_fold
     ok (low, high1)
 
 /-- [hachi::sumcheck::alpha_split_high]: loop body 0:
-    Source: 'src/sumcheck.rs', lines 920:4-923:5
+    Source: 'src/sumcheck.rs', lines 928:4-931:5
     Visibility: public -/
 @[rust_loop_body]
 def sumcheck.alpha_split_high_loop0.body
@@ -6882,7 +6880,7 @@ def sumcheck.alpha_split_high_loop0.body
   else ok (done k)
 
 /-- [hachi::sumcheck::alpha_split_high]: loop 0:
-    Source: 'src/sumcheck.rs', lines 920:4-923:5
+    Source: 'src/sumcheck.rs', lines 928:4-931:5
     Visibility: public -/
 @[rust_loop]
 def sumcheck.alpha_split_high_loop0
@@ -6894,7 +6892,7 @@ def sumcheck.alpha_split_high_loop0
     (k, sz)
 
 /-- [hachi::sumcheck::alpha_split_high]: loop body 2:
-    Source: 'src/sumcheck.rs', lines 932:8-937:9
+    Source: 'src/sumcheck.rs', lines 940:8-945:9
     Visibility: public -/
 @[rust_loop_body]
 def sumcheck.alpha_split_high_loop1_loop0.body
@@ -6926,7 +6924,7 @@ def sumcheck.alpha_split_high_loop1_loop0.body
   else ok (done sum)
 
 /-- [hachi::sumcheck::alpha_split_high]: loop 2:
-    Source: 'src/sumcheck.rs', lines 932:8-937:9
+    Source: 'src/sumcheck.rs', lines 940:8-945:9
     Visibility: public -/
 @[rust_loop]
 def sumcheck.alpha_split_high_loop1_loop0
@@ -6941,7 +6939,7 @@ def sumcheck.alpha_split_high_loop1_loop0
     (sum, i)
 
 /-- [hachi::sumcheck::alpha_split_high]: loop body 1:
-    Source: 'src/sumcheck.rs', lines 929:4-940:5
+    Source: 'src/sumcheck.rs', lines 937:4-948:5
     Visibility: public -/
 @[rust_loop_body]
 def sumcheck.alpha_split_high_loop1.body
@@ -6963,7 +6961,7 @@ def sumcheck.alpha_split_high_loop1.body
   else ok (done high)
 
 /-- [hachi::sumcheck::alpha_split_high]: loop 1:
-    Source: 'src/sumcheck.rs', lines 929:4-940:5
+    Source: 'src/sumcheck.rs', lines 937:4-948:5
     Visibility: public -/
 @[rust_loop]
 def sumcheck.alpha_split_high_loop1
@@ -6979,7 +6977,7 @@ def sumcheck.alpha_split_high_loop1
     (high, u)
 
 /-- [hachi::sumcheck::alpha_split_high]:
-    Source: 'src/sumcheck.rs', lines 909:0-942:1
+    Source: 'src/sumcheck.rs', lines 917:0-950:1
     Visibility: public -/
 def sumcheck.alpha_split_high
   (s : ringswitch.RlinStatement) (alpha : cpoly.field.Ext4)
@@ -7001,7 +6999,7 @@ def sumcheck.alpha_split_high
   sumcheck.alpha_split_high_loop1 rows cols hsz eqw mt high 0#usize
 
 /-- [hachi::sumcheck::alpha_split_low]: loop body 0:
-    Source: 'src/sumcheck.rs', lines 899:4-902:5
+    Source: 'src/sumcheck.rs', lines 907:4-910:5
     Visibility: public -/
 @[rust_loop_body]
 def sumcheck.alpha_split_low_loop.body
@@ -7018,7 +7016,7 @@ def sumcheck.alpha_split_low_loop.body
   else ok (done sz)
 
 /-- [hachi::sumcheck::alpha_split_low]: loop 0:
-    Source: 'src/sumcheck.rs', lines 899:4-902:5
+    Source: 'src/sumcheck.rs', lines 907:4-910:5
     Visibility: public -/
 @[rust_loop]
 def sumcheck.alpha_split_low_loop
@@ -7030,7 +7028,7 @@ def sumcheck.alpha_split_low_loop
     (k, sz)
 
 /-- [hachi::sumcheck::alpha_split_low]:
-    Source: 'src/sumcheck.rs', lines 895:0-904:1
+    Source: 'src/sumcheck.rs', lines 903:0-912:1
     Visibility: public -/
 def sumcheck.alpha_split_low
   (alpha : cpoly.field.Ext4) (m0 : Std.Usize) :
@@ -7041,7 +7039,7 @@ def sumcheck.alpha_split_low
   zerocheck.alpha_pow_table alpha sz
 
 /-- [hachi::sumcheck::eval_mle_layer_base]: loop body 0:
-    Source: 'src/sumcheck.rs', lines 737:4-742:5
+    Source: 'src/sumcheck.rs', lines 745:4-750:5
     Visibility: public -/
 @[rust_loop_body]
 def sumcheck.eval_mle_layer_base_loop.body
@@ -7070,7 +7068,7 @@ def sumcheck.eval_mle_layer_base_loop.body
   else ok (done out)
 
 /-- [hachi::sumcheck::eval_mle_layer_base]: loop 0:
-    Source: 'src/sumcheck.rs', lines 737:4-742:5
+    Source: 'src/sumcheck.rs', lines 745:4-750:5
     Visibility: public -/
 @[rust_loop]
 def sumcheck.eval_mle_layer_base_loop
@@ -7085,7 +7083,7 @@ def sumcheck.eval_mle_layer_base_loop
     (out, j)
 
 /-- [hachi::sumcheck::eval_mle_layer_base]:
-    Source: 'src/sumcheck.rs', lines 732:0-744:1
+    Source: 'src/sumcheck.rs', lines 740:0-752:1
     Visibility: public -/
 def sumcheck.eval_mle_layer_base
   (values : alloc.vec.Vec cpoly.field.Fp) (x0 : cpoly.field.Ext4) :
@@ -7099,7 +7097,7 @@ def sumcheck.eval_mle_layer_base
   sumcheck.eval_mle_layer_base_loop values x0 half one_minus out 0#usize
 
 /-- [hachi::sumcheck::honest_round_messages]: loop body 0:
-    Source: 'src/sumcheck.rs', lines 1560:8-1570:9
+    Source: 'src/sumcheck.rs', lines 1568:8-1578:9
     Visibility: public -/
 @[rust_loop_body]
 def sumcheck.honest_round_messages_loop.body
@@ -7129,7 +7127,7 @@ def sumcheck.honest_round_messages_loop.body
   else ok (done out)
 
 /-- [hachi::sumcheck::honest_round_messages]: loop 0:
-    Source: 'src/sumcheck.rs', lines 1560:8-1570:9
+    Source: 'src/sumcheck.rs', lines 1568:8-1578:9
     Visibility: public -/
 @[rust_loop]
 def sumcheck.honest_round_messages_loop
@@ -7147,7 +7145,7 @@ def sumcheck.honest_round_messages_loop
     (low, high, current, out, w_tab, i)
 
 /-- [hachi::sumcheck::honest_round_messages]:
-    Source: 'src/sumcheck.rs', lines 1534:0-1573:1
+    Source: 'src/sumcheck.rs', lines 1542:0-1581:1
     Visibility: public -/
 def sumcheck.honest_round_messages
   (stmt : sumcheck.RoundStatement) (w : ringswitch.LiftedWitness)
@@ -7179,7 +7177,7 @@ def sumcheck.honest_round_messages
   else ok (alloc.vec.Vec.new sumcheck.RoundMsg)
 
 /-- [hachi::sumcheck::honest_compute_y]:
-    Source: 'src/sumcheck.rs', lines 1385:0-1391:1
+    Source: 'src/sumcheck.rs', lines 1393:0-1399:1
     Visibility: public -/
 def sumcheck.honest_compute_y
   (w : ringswitch.LiftedWitness) (m0 : Std.Usize)
@@ -15653,7 +15651,7 @@ def sumcheck.round_values_zero
     cpoly.field.Ext4) 0#usize
 
 /-- [hachi::sumcheck::round_value_alpha]: loop body 0:
-    Source: 'src/sumcheck.rs', lines 486:4-491:5
+    Source: 'src/sumcheck.rs', lines 494:4-499:5
     Visibility: public -/
 @[rust_loop_body]
 def sumcheck.round_value_alpha_loop.body
@@ -15693,7 +15691,7 @@ def sumcheck.round_value_alpha_loop.body
   else ok (done acc)
 
 /-- [hachi::sumcheck::round_value_alpha]: loop 0:
-    Source: 'src/sumcheck.rs', lines 486:4-491:5
+    Source: 'src/sumcheck.rs', lines 494:4-499:5
     Visibility: public -/
 @[rust_loop]
 def sumcheck.round_value_alpha_loop
@@ -15708,7 +15706,7 @@ def sumcheck.round_value_alpha_loop
     (acc, y)
 
 /-- [hachi::sumcheck::round_value_alpha]:
-    Source: 'src/sumcheck.rs', lines 481:0-493:1
+    Source: 'src/sumcheck.rs', lines 489:0-501:1
     Visibility: public -/
 def sumcheck.round_value_alpha
   (w : alloc.vec.Vec cpoly.field.Ext4) (a_tab : alloc.vec.Vec cpoly.field.Ext4)
@@ -15724,7 +15722,7 @@ def sumcheck.round_value_alpha
     cpoly.field.Ext4.ZERO 0#usize
 
 /-- [hachi::sumcheck::round_values_alpha]: loop body 0:
-    Source: 'src/sumcheck.rs', lines 504:4-507:5
+    Source: 'src/sumcheck.rs', lines 512:4-515:5
     Visibility: public -/
 @[rust_loop_body]
 def sumcheck.round_values_alpha_loop.body
@@ -15743,7 +15741,7 @@ def sumcheck.round_values_alpha_loop.body
   else ok (done out)
 
 /-- [hachi::sumcheck::round_values_alpha]: loop 0:
-    Source: 'src/sumcheck.rs', lines 504:4-507:5
+    Source: 'src/sumcheck.rs', lines 512:4-515:5
     Visibility: public -/
 @[rust_loop]
 def sumcheck.round_values_alpha_loop
@@ -15757,7 +15755,7 @@ def sumcheck.round_values_alpha_loop
     (out, t)
 
 /-- [hachi::sumcheck::round_values_alpha]:
-    Source: 'src/sumcheck.rs', lines 500:0-509:1
+    Source: 'src/sumcheck.rs', lines 508:0-517:1
     Visibility: public -/
 @[reducible]
 def sumcheck.round_values_alpha
@@ -15769,7 +15767,7 @@ def sumcheck.round_values_alpha
     (alloc.vec.Vec.new cpoly.field.Ext4) 0#usize
 
 /-- [hachi::sumcheck::round_poly_alpha]:
-    Source: 'src/sumcheck.rs', lines 532:0-536:1
+    Source: 'src/sumcheck.rs', lines 540:0-544:1
     Visibility: public -/
 def sumcheck.round_poly_alpha
   (w : alloc.vec.Vec cpoly.field.Ext4) (a_tab : alloc.vec.Vec cpoly.field.Ext4)
@@ -15819,7 +15817,7 @@ def zerocheck.range_product_base
   zerocheck.range_product_base_loop params.GADGET_BASE c2 c 1#u64
 
 /-- [hachi::sumcheck::round_value_zero_base]: loop body 0:
-    Source: 'src/sumcheck.rs', lines 577:4-584:5
+    Source: 'src/sumcheck.rs', lines 585:4-592:5
     Visibility: public -/
 @[rust_loop_body]
 def sumcheck.round_value_zero_base_loop.body
@@ -15852,7 +15850,7 @@ def sumcheck.round_value_zero_base_loop.body
   else ok (done acc)
 
 /-- [hachi::sumcheck::round_value_zero_base]: loop 0:
-    Source: 'src/sumcheck.rs', lines 577:4-584:5
+    Source: 'src/sumcheck.rs', lines 585:4-592:5
     Visibility: public -/
 @[rust_loop]
 def sumcheck.round_value_zero_base_loop
@@ -15867,7 +15865,7 @@ def sumcheck.round_value_zero_base_loop
     (acc, y)
 
 /-- [hachi::sumcheck::round_value_zero_base]:
-    Source: 'src/sumcheck.rs', lines 572:0-586:1
+    Source: 'src/sumcheck.rs', lines 580:0-594:1
     Visibility: public -/
 def sumcheck.round_value_zero_base
   (w : alloc.vec.Vec cpoly.field.Fp) (eq : alloc.vec.Vec cpoly.field.Ext4)
@@ -15881,7 +15879,7 @@ def sumcheck.round_value_zero_base
     cpoly.field.Ext4.ZERO 0#usize
 
 /-- [hachi::sumcheck::round_values_zero_base]: loop body 0:
-    Source: 'src/sumcheck.rs', lines 598:4-601:5
+    Source: 'src/sumcheck.rs', lines 606:4-609:5
     Visibility: public -/
 @[rust_loop_body]
 def sumcheck.round_values_zero_base_loop.body
@@ -15901,7 +15899,7 @@ def sumcheck.round_values_zero_base_loop.body
   else ok (done out)
 
 /-- [hachi::sumcheck::round_values_zero_base]: loop 0:
-    Source: 'src/sumcheck.rs', lines 598:4-601:5
+    Source: 'src/sumcheck.rs', lines 606:4-609:5
     Visibility: public -/
 @[rust_loop]
 def sumcheck.round_values_zero_base_loop
@@ -15915,7 +15913,7 @@ def sumcheck.round_values_zero_base_loop
     (out, t)
 
 /-- [hachi::sumcheck::round_values_zero_base]:
-    Source: 'src/sumcheck.rs', lines 594:0-603:1
+    Source: 'src/sumcheck.rs', lines 602:0-611:1
     Visibility: public -/
 @[reducible]
 def sumcheck.round_values_zero_base
@@ -15926,7 +15924,7 @@ def sumcheck.round_values_zero_base
     (alloc.vec.Vec.new cpoly.field.Ext4) 0#usize
 
 /-- [hachi::sumcheck::round_value_alpha_base]: loop body 0:
-    Source: 'src/sumcheck.rs', lines 693:4-698:5
+    Source: 'src/sumcheck.rs', lines 701:4-706:5
     Visibility: public -/
 @[rust_loop_body]
 def sumcheck.round_value_alpha_base_loop.body
@@ -15968,7 +15966,7 @@ def sumcheck.round_value_alpha_base_loop.body
   else ok (done acc)
 
 /-- [hachi::sumcheck::round_value_alpha_base]: loop 0:
-    Source: 'src/sumcheck.rs', lines 693:4-698:5
+    Source: 'src/sumcheck.rs', lines 701:4-706:5
     Visibility: public -/
 @[rust_loop]
 def sumcheck.round_value_alpha_base_loop
@@ -15984,7 +15982,7 @@ def sumcheck.round_value_alpha_base_loop
     (acc, y)
 
 /-- [hachi::sumcheck::round_value_alpha_base]:
-    Source: 'src/sumcheck.rs', lines 686:0-700:1
+    Source: 'src/sumcheck.rs', lines 694:0-708:1
     Visibility: public -/
 def sumcheck.round_value_alpha_base
   (w : alloc.vec.Vec cpoly.field.Fp) (a_tab : alloc.vec.Vec cpoly.field.Ext4)
@@ -16003,7 +16001,7 @@ def sumcheck.round_value_alpha_base
     one_minus_ext cpoly.field.Ext4.ZERO 0#usize
 
 /-- [hachi::sumcheck::round_values_alpha_base]: loop body 0:
-    Source: 'src/sumcheck.rs', lines 708:4-711:5
+    Source: 'src/sumcheck.rs', lines 716:4-719:5
     Visibility: public -/
 @[rust_loop_body]
 def sumcheck.round_values_alpha_base_loop.body
@@ -16023,7 +16021,7 @@ def sumcheck.round_values_alpha_base_loop.body
   else ok (done out)
 
 /-- [hachi::sumcheck::round_values_alpha_base]: loop 0:
-    Source: 'src/sumcheck.rs', lines 708:4-711:5
+    Source: 'src/sumcheck.rs', lines 716:4-719:5
     Visibility: public -/
 @[rust_loop]
 def sumcheck.round_values_alpha_base_loop
@@ -16037,7 +16035,7 @@ def sumcheck.round_values_alpha_base_loop
     (out, t)
 
 /-- [hachi::sumcheck::round_values_alpha_base]:
-    Source: 'src/sumcheck.rs', lines 704:0-713:1
+    Source: 'src/sumcheck.rs', lines 712:0-721:1
     Visibility: public -/
 @[reducible]
 def sumcheck.round_values_alpha_base
@@ -16048,7 +16046,7 @@ def sumcheck.round_values_alpha_base
     (alloc.vec.Vec.new cpoly.field.Ext4) 0#usize
 
 /-- [hachi::sumcheck::round_poly_alpha_base]:
-    Source: 'src/sumcheck.rs', lines 717:0-721:1
+    Source: 'src/sumcheck.rs', lines 725:0-729:1
     Visibility: public -/
 def sumcheck.round_poly_alpha_base
   (w : alloc.vec.Vec cpoly.field.Fp) (a_tab : alloc.vec.Vec cpoly.field.Ext4) :
@@ -16059,7 +16057,7 @@ def sumcheck.round_poly_alpha_base
   sumcheck.interpolate values weights
 
 /-- [hachi::sumcheck::alpha_public_table]: loop body 1:
-    Source: 'src/sumcheck.rs', lines 790:8-795:9
+    Source: 'src/sumcheck.rs', lines 798:8-803:9
     Visibility: public -/
 @[rust_loop_body]
 def sumcheck.alpha_public_table_loop0_loop0.body
@@ -16091,7 +16089,7 @@ def sumcheck.alpha_public_table_loop0_loop0.body
   else ok (done sum)
 
 /-- [hachi::sumcheck::alpha_public_table]: loop 1:
-    Source: 'src/sumcheck.rs', lines 790:8-795:9
+    Source: 'src/sumcheck.rs', lines 798:8-803:9
     Visibility: public -/
 @[rust_loop]
 def sumcheck.alpha_public_table_loop0_loop0
@@ -16106,7 +16104,7 @@ def sumcheck.alpha_public_table_loop0_loop0
     (sum, i)
 
 /-- [hachi::sumcheck::alpha_public_table]: loop body 0:
-    Source: 'src/sumcheck.rs', lines 785:4-798:5
+    Source: 'src/sumcheck.rs', lines 793:4-806:5
     Visibility: public -/
 @[rust_loop_body]
 def sumcheck.alpha_public_table_loop0.body
@@ -16134,7 +16132,7 @@ def sumcheck.alpha_public_table_loop0.body
   else ok (done out)
 
 /-- [hachi::sumcheck::alpha_public_table]: loop 0:
-    Source: 'src/sumcheck.rs', lines 785:4-798:5
+    Source: 'src/sumcheck.rs', lines 793:4-806:5
     Visibility: public -/
 @[rust_loop]
 def sumcheck.alpha_public_table_loop0
@@ -16150,7 +16148,7 @@ def sumcheck.alpha_public_table_loop0
     (out, idx)
 
 /-- [hachi::sumcheck::alpha_public_table]:
-    Source: 'src/sumcheck.rs', lines 770:0-800:1
+    Source: 'src/sumcheck.rs', lines 778:0-808:1
     Visibility: public -/
 def sumcheck.alpha_public_table
   (s : ringswitch.RlinStatement) (alpha : cpoly.field.Ext4)
@@ -16171,14 +16169,14 @@ def sumcheck.alpha_public_table
     out 0#usize
 
 /-- [hachi::sumcheck::{hachi::sumcheck::NestedZeroCheckStmt}::t]:
-    Source: 'src/sumcheck.rs', lines 1144:4-1146:5
+    Source: 'src/sumcheck.rs', lines 1152:4-1154:5
     Visibility: public -/
 def sumcheck.NestedZeroCheckStmt.impl.t
   (self : sumcheck.NestedZeroCheckStmt) : Result linalg.PolyVec := do
   ok self.t
 
 /-- [hachi::sumcheck::{hachi::sumcheck::RoundMsg}::new]:
-    Source: 'src/sumcheck.rs', lines 1180:4-1182:5
+    Source: 'src/sumcheck.rs', lines 1188:4-1190:5
     Visibility: public -/
 def sumcheck.RoundMsg.new
   (g_zero : cpoly.univariate.UnivariatePoly)
@@ -16188,7 +16186,7 @@ def sumcheck.RoundMsg.new
   ok { g_zero, g_alpha }
 
 /-- [hachi::sumcheck::honest_compute_g]:
-    Source: 'src/sumcheck.rs', lines 1263:0-1278:1
+    Source: 'src/sumcheck.rs', lines 1271:0-1286:1
     Visibility: public -/
 def sumcheck.honest_compute_g
   (stmt : sumcheck.RoundStatement) (w_tab : alloc.vec.Vec cpoly.field.Ext4)
@@ -16213,7 +16211,7 @@ def sumcheck.honest_compute_g
   ok { g_zero, g_alpha }
 
 /-- [hachi::sumcheck::honest_compute_g_base]:
-    Source: 'src/sumcheck.rs', lines 1286:0-1300:1
+    Source: 'src/sumcheck.rs', lines 1294:0-1308:1
     Visibility: public -/
 def sumcheck.honest_compute_g_base
   (stmt : sumcheck.RoundStatement) (w_fp : alloc.vec.Vec cpoly.field.Fp)
@@ -16248,7 +16246,7 @@ def zerocheck.c_w_table_mle
   cpoly.multilinear.MultilinearEvals.from_values values
 
 /-- [hachi::sumcheck::round_loop]: loop body 0:
-    Source: 'src/sumcheck.rs', lines 1453:4-1465:1
+    Source: 'src/sumcheck.rs', lines 1461:4-1473:1
     Visibility: public -/
 @[rust_loop_body]
 def sumcheck.round_loop_loop.body
@@ -16280,7 +16278,7 @@ def sumcheck.round_loop_loop.body
   else ok (done (some current))
 
 /-- [hachi::sumcheck::round_loop]: loop 0:
-    Source: 'src/sumcheck.rs', lines 1453:4-1465:1
+    Source: 'src/sumcheck.rs', lines 1461:4-1473:1
     Visibility: public -/
 @[rust_loop]
 def sumcheck.round_loop_loop
@@ -16296,7 +16294,7 @@ def sumcheck.round_loop_loop
     (w_tab, a_tab, current, i)
 
 /-- [hachi::sumcheck::round_loop]:
-    Source: 'src/sumcheck.rs', lines 1438:0-1465:1
+    Source: 'src/sumcheck.rs', lines 1446:0-1473:1
     Visibility: public -/
 def sumcheck.round_loop
   (stmt : sumcheck.RoundStatement) (w : ringswitch.LiftedWitness)
